More progress on blake2_update_multi

code/hash/Hacl.Hash.Blake2.fst
@@ -1,8 +1,11 @@
 module Hacl.Hash.Blake2
 
 module B = LowStar.Buffer
+module HS = FStar.HyperStack
 module ST = FStar.HyperStack.ST
 module M = LowStar.Modifies
+module S = FStar.Seq
+module U32 = FStar.UInt32
 
 open Lib.IntTypes
 
@@ -10,18 +13,63 @@ module Spec = Spec.Blake2
 module Impl = Hacl.Impl.Blake2.Generic
 module Core = Hacl.Impl.Blake2.Core
 
+open Hacl.Hash.Lemmas
+open Spec.Blake2.Lemmas
+
 open FStar.Mul
 
 #set-options "--fuel 0 --ifuel 0"
 
-#push-options "--fuel 1 --ifuel 1"
+#push-options "--fuel 1 --ifuel 1 --z3rlimit 50"
 
 noextract inline_for_extraction
 val mk_update_multi: a:hash_alg{is_blake a} -> update:update_st a -> update_multi_st a
 
-let mk_update_multi a update s ev block n_blocks =
+let mk_update_multi a update s ev blocks n_blocks =
   let h0 = ST.get () in
-  admit()
+  let inv (h: HS.mem) (i: nat) =
+    let i_block = block_length a * i in
+    let i_block' = block_length a * (i+1) in
+    i <= U32.v n_blocks /\
+    B.live h s /\ B.live h blocks /\
+    B.(modifies (loc_buffer s) h0 h) /\
+    (as_seq h s, add_extra_i a ev (U32.uint_to_t i)) ==
+      (Spec.Agile.Hash.update_multi a (as_seq h0 s, ev) (S.slice (B.as_seq h0 blocks) 0 i_block))
+  in
+  let f (i:U32.t { U32.(0 <= v i /\ v i < v n_blocks)}): ST.Stack unit
+    (requires (fun h -> inv h (U32.v i)))
+    (ensures (fun h0 _ h1 -> inv h0 (U32.v i) /\ inv h1 (U32.v i + 1)))
+  =
+    let h1 = ST.get () in
+    let sz = block_len a in
+    let blocks0 = B.sub blocks 0ul U32.(sz *^ i) in
+    let block = B.sub blocks U32.(sz *^ i) sz in
+    let v' = update s (add_extra_i a ev i) block in
+    let h2 = ST.get () in
+    let aux () : Lemma ((as_seq h2 s, v') ==
+      Spec.Agile.Hash.update_multi a (as_seq h0 s, ev) (S.slice (B.as_seq h0 blocks) 0 (block_length a * (U32.v i + 1))) /\
+      v' == add_extra_i a ev (U32.uint_to_t (U32.v i + 1))
+      )
+    = let s0 = as_seq h0 s in
+      let s1 = as_seq h1 s in
+      let blocks = B.as_seq h0 blocks in
+      let block = B.as_seq h0 block in
+      let i = U32.v i in
+      let i_block = block_length a * i in
+      let i_block' = block_length a * (i + 1) in
+      let blocks1:bytes_blocks a = S.slice blocks 0 i_block in
+      let blocks2:bytes_blocks a = S.slice blocks i_block i_block' in
+      let s_blocks:bytes_blocks a = S.slice blocks 0 i_block' in
+      Spec.Hash.Lemmas.update_multi_update a (s1, ev) block;
+      Spec.Hash.Lemmas.update_multi_associative a (s0, ev) blocks1 blocks2;
+      update_multi_add_extra a (s0, ev) (i+1) s_blocks
+    in aux ()
+  in
+  (**) assert (B.length blocks = U32.v n_blocks * block_length a);
+  (**) add_extra_i_zero a ev;
+  C.Loops.for 0ul n_blocks inv f;
+  add_extra_i a ev n_blocks
+
 
 #pop-options
 
