specs/lemmas/Spec.Blake2.Lemmas.fst
@@ -1,0 +1,133 @@
+module Spec.Blake2.Lemmas
+
+open Lib.IntTypes
+
+open Spec.Hash.Lemmas
+open Lib.UpdateMulti
+open FStar.Mul
+
+friend Spec.Agile.Hash
+
+
+#push-options "--fuel 0 --ifuel 0"
+
+noextract inline_for_extraction
+let add_extra_i (a:hash_alg{is_blake a}) (ev:extra_state a) (i:U32.t) : extra_state a =
+  match a with
+  | Blake2S ->
+    [@inline_let] let s = to_u64 i *. u64 (size_block a) in
+    ev +. s
+  | Blake2B -> admit()
+    // [@inline_let] let s = to_u128 i *. u128 (size_block a) in
+    // ev +. s
+
+let add_extra_s (a:hash_alg{is_blake a}) (ev:nat) (i:nat) : nat =
+  match a with
+  | Blake2S -> (ev + (i * size_block a)) % pow2 64
+  | Blake2B -> admit()
+
+let add_s_i_2s (ev:extra_state Blake2S) (i:U32.t) : Lemma
+  (v (add_extra_i Blake2S ev i) == add_extra_s Blake2S (v ev) (v i))
+  = calc (==) {
+      v (add_extra_i Blake2S ev i);
+      (==) { }
+      v (ev +. (to_u64 i *. u64 (size_block Blake2S)));
+      (==) { }
+      (v ev + (v i * size_block Blake2S) % pow2 64) % pow2 64;
+      (==) { FStar.Math.Lemmas.lemma_mod_add_distr (v ev) (v i * size_block Blake2S) (pow2 64) }
+      (v ev + v i * size_block Blake2S) % pow2 64;
+    }
+
+let add_extra_s_zero_2s (ev:extra_state Blake2S) : Lemma (add_extra_s Blake2S (v ev) 0 == v ev)
+  = ()
+
+let add_extra_i_zero a ev = match a with
+  | Blake2S ->
+    add_s_i_2s ev 0ul;
+    add_extra_s_zero_2s ev
+
+  | Blake2B -> admit()
+
+let add_extra_s_assoc_2s (ev:nat) (i j:nat) : Lemma
+  (add_extra_s Blake2S (add_extra_s Blake2S ev j) i == add_extra_s Blake2S ev (i + j))
+  = calc (==) {
+      add_extra_s Blake2S (add_extra_s Blake2S ev j) i;
+      (==) { }
+      ((add_extra_s Blake2S ev j) + (i * size_block Blake2S)) % pow2 64;
+      (==) { }
+      ((ev + (j * size_block Blake2S)) % pow2 64 + (i * size_block Blake2S)) % pow2 64;
+      (==) { FStar.Math.Lemmas.lemma_mod_add_distr (i * size_block Blake2S)
+        (ev + (j * size_block Blake2S)) (pow2 64) }
+      (ev + i * size_block Blake2S + j * size_block Blake2S) % pow2 64;
+      (==) { FStar.Math.Lemmas.distributivity_add_left i j (size_block Blake2S) }
+      add_extra_s Blake2S ev (i+j);
+   }
+
+
+val aux_2s (h:words_state Blake2S) (i:nat) (input: bytes_blocks Blake2S) :
+  Lemma (requires i + 1 < pow2 32 /\ Seq.length input == i * block_length Blake2S)
+        (ensures (
+          let h' = update_multi Blake2S h input in
+          v (snd h') == add_extra_s Blake2S (v (snd h)) i))
+        (decreases i)
+
+
+val update1_add (h:words_state Blake2S) (l:bytes{Seq.length l == block_length Blake2S})
+  : Lemma
+  (let h' = update Blake2S h l in
+   let _, ev = h in
+   let _, ev' = h' in
+   ev' == add_extra_i Blake2S ev 1ul)
+let update1_add h l =
+  mul_mod_lemma (to_u64 1ul) (u64 (size_block Blake2S))
+
+#restart-solver
+#push-options "--fuel 1 --z3rlimit 20"
+
+let rec aux_2s h i input =
+  let ev = snd h in
+  let h' = update_multi Blake2S h input in
+  let ev' = snd h' in
+  if i = 0 then add_extra_s_zero_2s ev
+  else
+    let block, rem = split_block (block_length Blake2S) input 1 in
+    let h_mid = update Blake2S h block in
+    let h_f = update_multi Blake2S h_mid rem in
+
+    let ev_mid = snd h_mid in
+    let ev_f = snd h_f in
+
+    calc (==) {
+      v ev';
+      (==) { }
+      v ev_f;
+      (==) { aux_2s h_mid (i-1) rem }
+      add_extra_s Blake2S (v ev_mid) (i-1);
+      (==) { update1_add h block }
+      add_extra_s Blake2S (v (add_extra_i Blake2S ev 1ul)) (i-1);
+      (==) { calc (==) {
+        v (add_extra_i Blake2S ev 1ul);
+        (==) { add_s_i_2s ev 1ul }
+        add_extra_s Blake2S (v ev) 1;
+          }
+        }
+      add_extra_s Blake2S (add_extra_s Blake2S (v ev) 1) (i-1);
+      (==) { add_extra_s_assoc_2s (v ev) (i-1) 1 }
+      add_extra_s Blake2S (v ev) i;
+    }
+
+#pop-options
+
+
+let rec update_multi_add_extra a h i input =
+  let ev = snd h in
+  let h' = update_multi a h input in
+  let ev' = snd h' in
+  match a with
+  | Blake2S ->
+    add_s_i_2s ev (U32.uint_to_t i);
+    aux_2s h i input
+
+  | Blake2B -> admit()
+
+#pop-options
