specs/lemmas/Spec.Blake2.Lemmas.fsti
@@ -1,0 +1,25 @@
+module Spec.Blake2.Lemmas
+
+module U32 = FStar.UInt32
+
+open Spec.Hash.Definitions
+open Spec.Agile.Hash
+open FStar.Mul
+
+noextract inline_for_extraction
+val add_extra_i (a:hash_alg{is_blake a}) (ev:extra_state a) (i:U32.t) : extra_state a
+
+val add_extra_i_zero (a:hash_alg{is_blake a}) (ev:extra_state a):
+  Lemma (add_extra_i a ev 0ul == ev)
+
+val update_multi_add_extra (a:hash_alg{is_blake a})
+  (h: words_state a)
+  (i:nat)
+  (input: bytes_blocks a):
+  Lemma
+  (requires i + 1 < pow2 32 /\ Seq.length input = block_length a * i)
+  (ensures
+    (
+     let h' = update_multi a h input in
+     snd h' == add_extra_i a (snd h) (U32.uint_to_t i)))
+  (decreases i)
